# O-RIM (Ontological RIM_) definitions
# This is work in progress, and may change rapidly 

@prefix dc: <http://purl.org/dc/elements/1.1/> .
@prefix dcterms: <http://purl.org/dc/terms/> .
@prefix owl: <http://www.w3.org/2002/07/owl#> .
@prefix rdf: <http://www.w3.org/1999/02/22-rdf-syntax-ns#> .
@prefix rdfs: <http://www.w3.org/1999/02/22-rdf-syntax-ns#> .
@prefix rim: <http://hl7.org/orim/class/> .
@prefix dt: <http://hl7.org/orim/datatype/> .
@prefix vs: <http://hl7.org/orim/valueset/> .
@prefix cs: <http://hl7.org/orim/codesystem/> .
@prefix xs: <http://www.w3.org/2001/XMLSchema/> .
@prefix fhir: <http://hl7.org/fhir/> .

# - ANY --------------------------------------------------------------------

dt:ANY a rdfs:Class;
   rdfs:subClassOf [
     a owl:Restriction;
     owl:onProperty dt:ANY.nullFlavor;
     owl:maxCardinality "1^^xs:nonNegativeInteger"
   ];
   dc:terms " An abstract type that defines the basic properties common to all data values defined in this specification. Data Value is an abstract type, meaning that no proper value can be just a data value without belonging to any concrete type. Every concrete type is a specialization of this general abstract DataValue type";
   dc:title "Base Data type";
   rdfs:comment "An abstract type that defines the basic properties common to all data values defined in this specification. Data Value is an abstract type, meaning that no proper value can be just a data value without belonging to any concrete type. Every concrete type is a specialization of this general abstract DataValue type";
   rdfs:label "Base Data type".

dt:ANY.nullFlavor a rdf:Property;
   dc:terms "An indicator of a data value's exceptional status, sometimes also denoting the manner and rationale for that status.";
   fhir:maxCardinality "1";
   fhir:minCardinality "0";
   rdfs:comment "An indicator of a data value's exceptional status, sometimes also denoting the manner and rationale for that status.";
   rdfs:domain dt:ANY;
   rdfs:range cs:NullFlavor.class;
   fhir:binding vs:NullFlavor;
   fhir:bindingStrength fhir:BindingStrength\#required.

# - CS ------------------------------------------------------------------

dt:CS rdfs:subClassOf dt:ANY;
   rdfs:subClassOf [
     a owl:Restriction;
     owl:onProperty dt:CS.code;
     owl:maxCardinality "1^^xs:nonNegativeInteger"
   ];
   dcterms:description "Coded data in its simplest form, where only the code is not predetermined. The code system and code system version are fixed by the context in which CS value occurs. CS is used for coded attributes that have a single HL7-defined value set";
   dc:title "CodedSimpleValue";
   rdfs:comment "Coded data in its simplest form, where only the code is not predetermined. The code system and code system version are fixed by the context in which CS value occurs. CS is used for coded attributes that have a single HL7-defined value set";
   rdfs:label "CodedSimpleValue".

dt:CS.code a rdf:Property;
   fhir:maxCardinality "1";
   fhir:minCardinality "0";
   rdfs:domain dt:CS;
   rdfs:range xs:string.

# - CD ------------------------------------------------------------------

#CD has been restructured in the oRIM to make reasoning easy.

dt:CD rdfs:subClassOf dt:ANY;
   rdfs:subClassOf [
     a owl:Restriction;
     owl:onProperty dt:II.originalText;
     owl:maxCardinality "1^^xs:nonNegativeInteger"
   ];
   dc:title "ConceptDescriptor";
   dcterms:description "A concept defined by text and/or references to concepts defined in a code system";
   rdfs:comment "A concept defined by text and/or references to concepts defined in a code system";
   rdfs:label "ConceptDescriptor".

dt:CD.coding a rdf:Property;
   dcterms:description "A reference to a concept defined in a code system";
   rdfs:comment "A reference to a concept defined in a code system";
   fhir:maxCardinality "*";
   fhir:minCardinality "0";
   rdfs:domain dt:CD;
   rdfs:range xs:string.

dt:CD.originalText a rdf:Property;
   dcterms:description "The text as seen and/or selected by the user who entered the data which represents the intended meaning of the user";
   rdfs:comment "The text as seen and/or selected by the user who entered the data which represents the intended meaning of the user";
   fhir:maxCardinality "1";
   fhir:minCardinality "0";
   rdfs:domain dt:CD;
   rdfs:range xs:string. # todo: dt:ED.TEXT.
 
dt:CDCoding rdfs:subClassOf dt:ANY;
   rdfs:subClassOf [
     a owl:Restriction;
     owl:onProperty dt:II.code;
     owl:maxCardinality "1^^xs:nonNegativeInteger"
   ];
   rdfs:subClassOf [
     a owl:Restriction;
     owl:onProperty dt:II.codeSystem;
     owl:maxCardinality "1^^xs:nonNegativeInteger"
   ];
   rdfs:subClassOf [
     a owl:Restriction;
     owl:onProperty dt:II.codeSystemName;
     owl:maxCardinality "1^^xs:nonNegativeInteger"
   ];
   rdfs:subClassOf [
     a owl:Restriction;
     owl:onProperty dt:II.codeSystemVersion;
     owl:maxCardinality "1^^xs:nonNegativeInteger"
   ];
   rdfs:subClassOf [
     a owl:Restriction;
     owl:onProperty dt:II.valueSet;
     owl:maxCardinality "1^^xs:nonNegativeInteger"
   ];
   rdfs:subClassOf [
     a owl:Restriction;
     owl:onProperty dt:II.valueSetVersion;
     owl:maxCardinality "1^^xs:nonNegativeInteger"
   ];
   rdfs:subClassOf [
     a owl:Restriction;
     owl:onProperty dt:II.displayName;
     owl:maxCardinality "1^^xs:nonNegativeInteger"
   ];
   rdfs:subClassOf [
     a owl:Restriction;
     owl:onProperty dt:II.originalText;
     owl:maxCardinality "1^^xs:nonNegativeInteger"
   ];
   rdfs:subClassOf [
     a owl:Restriction;
     owl:onProperty dt:II.source;
     owl:maxCardinality "1^^xs:nonNegativeInteger"
   ];
   dc:title "ConceptDescriptorCoding";
   dcterms:description "A reference to a concept defined in a code system";
   rdfs:comment "A reference to a concept defined in a code system";
   rdfs:label "ConceptDescriptorCoding".

dt:CDCoding.code a rdf:Property;
   dcterms:description "The plain code symbol defined by the code system, or an expression in a syntax defined by the code system which describes the concept";
   rdfs:comment "The plain code symbol defined by the code system, or an expression in a syntax defined by the code system which describes the concept";
   fhir:maxCardinality "1";
   fhir:minCardinality "0";
   rdfs:domain dt:CDCoding;
   rdfs:range xs:string.

dt:CDCoding.codeSystem a rdf:Property;
   dcterms:description "The code system that defines the code";
   rdfs:comment "The code system that defines the code";
   fhir:maxCardinality "1";
   fhir:minCardinality "0";
   rdfs:domain dt:CDCoding;
   rdfs:range xs:string.
   # in the RIM proper this must be an OID or a UUID. But for the o-RIM, we are primarily interested in statements or meaning, so we allow URL as well
   # owl:withRestriction [ xs:pattern "((0|[1-9][0-9]*)(\\.(0|[1-9][0-9]*)))|([0-9a-f]{8}-[0-9a-f]{4}-[0-9a-f]{4}-[0-9a-f]{4}-[0-9a-f]{12})|((http(s)?:\/\/.)?(www\.)?[-a-zA-Z0-9@:%._\+~#=]{2,256}\.[a-z]{2,6}\b([-a-zA-Z0-9@:%_\+.~#?&//=]*))"].
   
dt:CDCoding.codeSystemName a rdf:Property;
   dcterms:description "The common name of the coding system";
   rdfs:comment "The common name of the coding system";
   fhir:maxCardinality "1";
   fhir:minCardinality "0";
   rdfs:domain dt:CDCoding;
   rdfs:range xs:string.
 
dt:CDCoding.codeSystemVersion a rdf:Property;
   dcterms:description "If applicable, a version descriptor defined specifically for the given code system";
   rdfs:comment "If applicable, a version descriptor defined specifically for the given code system";
   fhir:maxCardinality "1";
   fhir:minCardinality "0";
   rdfs:domain dt:CDCoding;
   rdfs:range xs:string.
 
dt:CDCoding.valueSet a rdf:Property;
   dcterms:description "The value set that applied when this CD was created";
   rdfs:comment "The value set that applied when this CD was created";
   fhir:maxCardinality "1";
   fhir:minCardinality "0";
   rdfs:domain dt:CDCoding;
   rdfs:range xs:string.
 
dt:CDCoding.valueSetVersion a rdf:Property;
   dcterms:description "The version of the value set that applied when this CD was created";
   rdfs:comment "The version of the value set that applied when this CD was created";
   fhir:maxCardinality "1";
   fhir:minCardinality "0";
   rdfs:domain dt:CDCoding;
   rdfs:range xs:string.
 
dt:CDCoding.displayName a rdf:Property;
   dcterms:description "A name, title, or representation for the code or expression as it exists in the code system identified by the value of codeSystem";
   rdfs:comment "A name, title, or representation for the code or expression as it exists in the code system identified by the value of codeSystem.";
   fhir:maxCardinality "1";
   fhir:minCardinality "0";
   rdfs:domain dt:CDCoding;
   rdfs:range xs:string.
 
dt:CDCoding.codingRationale a rdf:Property;
   dcterms:description "The reason a particular CD has been provided";
   rdfs:comment "The reason a particular CD has been provided";
   fhir:maxCardinality "*";
   fhir:minCardinality "0";
   rim:collectionType rim:CollectionType\#DSET;
   rdfs:domain dt:CDCoding;
   rdfs:range cs:CodingRationale.class;
   fhir:binding vs:CodingRationale;
   fhir:bindingStrength fhir:BindingStrength\#required.
      
dt:CDCoding.source a rdf:Property;
   dcterms:description "The CD from which this CD was translated, if it was translated from another CD";
   rdfs:comment "The CD from which this CD was translated, if it was translated from another CD";
   fhir:maxCardinality "1";
   fhir:minCardinality "0";
   rdfs:domain dt:CDCoding;
   rdfs:range dt:CDCoding.
   
   
# - II ------------------------------------------------------------------

dt:II rdfs:subClassOf dt:ANY;
   rdfs:subClassOf [
     a owl:Restriction;
     owl:onProperty dt:II.root;
     owl:maxCardinality "1^^xs:nonNegativeInteger"
   ];
   rdfs:subClassOf [
     a owl:Restriction;
     owl:onProperty dt:II.extension;
     owl:maxCardinality "1^^xs:nonNegativeInteger"
   ];
   rdfs:subClassOf [
     a owl:Restriction;
     owl:onProperty dt:II.identifierName;
     owl:maxCardinality "1^^xs:nonNegativeInteger"
   ];
   rdfs:subClassOf [
     a owl:Restriction;
     owl:onProperty dt:II.scope;
     owl:maxCardinality "1^^xs:nonNegativeInteger"
   ];
   rdfs:subClassOf [
     a owl:Restriction;
     owl:onProperty dt:II.reliability;
     owl:maxCardinality "1^^xs:nonNegativeInteger"
   ];
   rdfs:subClassOf [
     a owl:Restriction;
     owl:onProperty dt:II.display;
     owl:maxCardinality "1^^xs:nonNegativeInteger"
   ];
   dc:title "InstanceIdentifier";
   dcterms:description "An identifier that uniquely identifies a thing or object. Examples are object identifier for HL7 RIM objects, medical record number, order id, service catalog item id, Vehicle Identification Number (VIN), etc.";
   rdfs:comment "An identifier that uniquely identifies a thing or object. Examples are object identifier for HL7 RIM objects, medical record number, order id, service catalog item id, Vehicle Identification Number (VIN), etc.";
   rdfs:label "InstanceIdentifier".

dt:II.root a rdf:Property;
   dcterms:description "A unique identifier that guarantees the global uniqueness of the instance identifier. The root alone may be the entire instance identifier";
   rdfs:comment "A unique identifier that guarantees the global uniqueness of the instance identifier. The root alone may be the entire instance identifier";
   fhir:maxCardinality "1";
   fhir:minCardinality "0";
   rdfs:domain dt:II;
   rdfs:range xs:string.
   # in the RIM proper this must be an OID or a UUID. But for the o-RIM, we are primarily interested in statements or meaning, so we allow URL as well
   # owl:withRestriction [ xs:pattern "((0|[1-9][0-9]*)(\\.(0|[1-9][0-9]*)))|([0-9a-f]{8}-[0-9a-f]{4}-[0-9a-f]{4}-[0-9a-f]{4}-[0-9a-f]{12})|((http(s)?:\/\/.)?(www\.)?[-a-zA-Z0-9@:%._\+~#=]{2,256}\.[a-z]{2,6}\b([-a-zA-Z0-9@:%_\+.~#?&//=]*))"].
   
dt:II.extension a rdf:Property;
   dcterms:description "A character string as a unique identifier within the scope of the identifier root.";
   rdfs:comment "A character string as a unique identifier within the scope of the identifier root.";
   fhir:maxCardinality "1";
   fhir:minCardinality "0";
   rdfs:domain dt:II;
   rdfs:range xs:string.

dt:II.identifierName a rdf:Property;
   dcterms:description "This is a human-readable name for the namespace represented in the root. It is a descriptive name for the actual namespace. e.g. 'California, U.S. Driver's License Number, 1970-'.";
   rdfs:comment "This is a human-readable name for the namespace represented in the root. It is a descriptive name for the actual namespace. e.g. 'California, U.S. Driver's License Number, 1970-'.";
   fhir:maxCardinality "1";
   fhir:minCardinality "0";
   rdfs:domain dt:II;
   rdfs:range xs:string.
 
dt:II.scope a rdf:Property;
   dcterms:description "Specifies the scope in which the identifier applies to the object with which it is associated";
   rdfs:comment "Specifies the scope in which the identifier applies to the object with which it is associated";
   fhir:maxCardinality "1";
   fhir:minCardinality "0";
   rdfs:domain dt:II;
   rdfs:range cs:IdentifierScope.class;
   fhir:binding vs:IdentifierScope;
   fhir:bindingStrength fhir:BindingStrength\#required.

dt:II.reliability a rdf:Property;
   dcterms:description "Specifies the reliability with which the identifier is known. This attribute MAY be used to assist with identifier matching algorithms";
   rdfs:comment "Specifies the reliability with which the identifier is known. This attribute MAY be used to assist with identifier matching algorithms";
   fhir:maxCardinality "1";
   fhir:minCardinality "0";
   rdfs:domain dt:II;
   rdfs:range cs:IdentifierReliability.class;
   fhir:binding vs:IdentifierReliability;
   fhir:bindingStrength fhir:BindingStrength\#required.
   
dt:II.display a rdf:Property;
   dcterms:description "Specifies if the identifier is intended for human display and data entry (displayable = true) as opposed to pure machine interoperation (displayable = false)";
   rdfs:comment "Specifies if the identifier is intended for human display and data entry (displayable = true) as opposed to pure machine interoperation (displayable = false)";
   fhir:maxCardinality "1";
   fhir:minCardinality "0";
   rdfs:domain dt:II;
   rdfs:range xs:boolean.
   
      
# - InfrastructureRoot --------------------------------------------------------------------

rim:InfrastructureRoot a rdfs:Class;
   rdfs:subClassOf [
     a owl:Restriction;
     owl:onProperty rim:InfrastructureRoot.nullFlavor;
     owl:maxCardinality "1^^xs:nonNegativeInteger"
   ];
   dcterms:description "An abstract super-type for all RIM classes, either directly or through inheritance";
   dc:title "Base RIM Class";
   rdfs:comment "An abstract super-type for all RIM classes, either directly or through inheritance";
   rdfs:label "Base RIM Class".

rim:InfrastructureRoot.nullFlavor a rdf:Property;
   dcterms:description "An indicator that the class instance is null, including the flavor of null that is intended";
   fhir:maxCardinality "1";
   fhir:minCardinality "0";
   rdfs:comment "An indicator that the class instance is null, including the flavor of null that is intended";
   rdfs:domain rim:InfrastructureRoot;
   rdfs:range dt:CS;
   fhir:binding vs:NullFlavor;
   fhir:bindingStrength fhir:BindingStrength\#required.
   
# - Entity --------------------------------------------------------------------

rim:Entity rdfs:subClassOf rim:InfrastructureRoot;
   rdfs:subClassOf [
     a owl:Restriction;
     owl:onProperty rim:Entity.classCode;
     owl:maxCardinality "1^^xs:nonNegativeInteger"
   ];
   rdfs:subClassOf [
     a owl:Restriction;
     owl:onProperty rim:Entity.classCode;
     owl:minCardinality "1^^xs:nonNegativeInteger"
   ];
   rdfs:subClassOf [
     a owl:Restriction;
     owl:onProperty rim:Entity.determinerCode;
     owl:maxCardinality "1^^xs:nonNegativeInteger"
   ];
   rdfs:subClassOf [
     a owl:Restriction;
     owl:onProperty rim:Entity.determinerCode;
     owl:minCardinality "1^^xs:nonNegativeInteger"
   ];
   rdfs:subClassOf [
     a owl:Restriction;
     owl:onProperty rim:Entity.statusCode;
     owl:maxCardinality "1^^xs:nonNegativeInteger"
   ];
   rdfs:subClassOf [
     a owl:Restriction;
     owl:onProperty rim:Entity.code;
     owl:maxCardinality "1^^xs:nonNegativeInteger"
   ];
   dcterms:description "A physical thing, group of physical things or an organization capable of participating in Acts while in a role";
   dc:title "Entity";
   rdfs:comment "A physical thing, group of physical things or an organization capable of participating in Acts while in a role";
   rdfs:label "Entity".
 
rim:Entity.classCode a rdf:Property;
   dcterms:description "The major class of Entities to which an Entity-instance belongs";
   fhir:maxCardinality "1";
   fhir:minCardinality "1";
   rdfs:comment "The major class of Entities to which an Entity-instance belongs";
   rdfs:domain rim:Entity;
   rdfs:range cs:EntityClass.class;
   fhir:binding vs:EntityClass;
   fhir:bindingStrength fhir:BindingStrength\#required.
   
rim:Entity.determinerCode a rdf:Property;
   dcterms:description "A code specifying whether the Entity object represents a universal (KIND) vs. a particular (INSTANCE)";
   fhir:maxCardinality "1";
   fhir:minCardinality "1";
   rdfs:comment "A code specifying whether the Entity object represents a universal (KIND) vs. a particular (INSTANCE)";
   rdfs:domain rim:Entity;
   rdfs:range cs:EntityDeterminer.class;
   fhir:binding vs:EntityDeterminer;
   fhir:bindingStrength fhir:BindingStrength\#required.
   
rim:Entity.statusCode a rdf:Property;
   dcterms:description "A value representing whether the information associated with an Entity is currently active or inactive for the purpose of participation in acts";
   fhir:maxCardinality "1";
   fhir:minCardinality "0";
   rdfs:comment "A value representing whether the information associated with an Entity is currently active or inactive for the purpose of participation in acts";
   rdfs:domain rim:Entity;
   rdfs:range cs:EntityStatus.class;
   fhir:binding vs:EntityStatus;
   fhir:bindingStrength fhir:BindingStrength\#required.

rim:Entity.id a rdf:Property;
   dcterms:description "A unique identifier for the Entity";
   fhir:maxCardinality "*";
   fhir:minCardinality "0";
   rim:collectionType rim:CollectionType\#DSET;
   rdfs:comment "A unique identifier for the Entity";
   rdfs:domain rim:Entity;
   rdfs:range dt:II.
   
rim:Entity.code a rdf:Property;
   dcterms:description "The specific kind of Entity to which an Entity-instance belongs";
   fhir:maxCardinality "1";
   fhir:minCardinality "0";
   rim:collectionType rim:CollectionType\#DSET;
   rdfs:comment "The specific kind of Entity to which an Entity-instance belongs";
   rdfs:domain rim:Entity;
   rdfs:range dt:CD;
   fhir:binding vs:EntityCode;
   fhir:bindingStrength fhir:BindingStrength\#extensible.
   
   
#- for all classes mapped to acts, we know what happened to classCode, moodCode, code, negationInd,x2, statusCode, id
#- for all classes mapped to roles, we know what happened to classCode, statusCode, code, negationInd, id, and player,
#- for all classes mapped to entities, we know what happened to classCode, determineCode, id, code, statusCode   


cs:NullFlavor\#NIclass rdfs:subClassOf cs:NullFlavor ;
  owl:oneOf (cs:NullFlavor\#NI cs:NullFlavor\#OTH).
  
cs:NullFlavor\#OTHclass rdfs:subClassOf cs:NullFlavor\#NIclass ; 
  owl:oneOf (cs:NullFlavor\#OTH).

# - vs:NullFlavor --------------------------------------------------------------

vs:NullFlavor a fhir:ValueSet;
  fhir:version "2015-03-23";
  rdfs:label "v3 Code System NullFlavor";
  dc:title "v3 Code System NullFlavor";
  rdfs:comment " A collection of codes specifying why a valid value is not present.";
  dcterms:description " A collection of codes specifying why a valid value is not present.";
  dc:date "Mon Mar 23 00:00:00 EST 2015";
  fhir:status fhir:conformance-resource-status\#active;
  fhir:canonical-status fhir:canonical-status-codes\#active;
  fhir:include cs:NullFlavor.

cs:NullFlavor a fhir:CodeSystem;
  rdfs:label "v3 Code System NullFlavor";
  dc:title "v3 Code System NullFlavor";
  rdfs:comment " A collection of codes specifying why a valid value is not present.";
  dcterms:description " A collection of codes specifying why a valid value is not present.";
  dc:date "Mon Mar 23 00:00:00 EST 2015";
  fhir:conceptList cs:NullFlavor.class.

cs:NullFlavor.class a fhir:Concept;
  owl:oneOf (cs:NullFlavor\#NI cs:NullFlavor\#INV cs:NullFlavor\#DER cs:NullFlavor\#OTH cs:NullFlavor\#NINF cs:NullFlavor\#PINF cs:NullFlavor\#UNC cs:NullFlavor\#MSK cs:NullFlavor\#NA cs:NullFlavor\#UNK cs:NullFlavor\#ASKU cs:NullFlavor\#NAV cs:NullFlavor\#NASK cs:NullFlavor\#QS cs:NullFlavor\#TRC).

cs:NullFlavor.class\#NI rdfs:subClassOf cs:NullFlavor.class;
  owl:oneOf (cs:NullFlavor\#NI cs:NullFlavor\#INV cs:NullFlavor\#DER cs:NullFlavor\#OTH cs:NullFlavor\#NINF cs:NullFlavor\#PINF cs:NullFlavor\#UNC cs:NullFlavor\#MSK cs:NullFlavor\#NA cs:NullFlavor\#UNK cs:NullFlavor\#ASKU cs:NullFlavor\#NAV cs:NullFlavor\#NASK cs:NullFlavor\#QS cs:NullFlavor\#TRC);
  rdfs:label "NoInformation";
  dc:title "NoInformation";
  rdfs:comment "Description:The value is exceptional (missing, omitted, incomplete, improper). No information as to the reason for being an exceptional value is provided. This is the most general exceptional value. It is also the default exceptional value.";
  dcterms:description "Description:The value is exceptional (missing, omitted, incomplete, improper). No information as to the reason for being an exceptional value is provided. This is the most general exceptional value. It is also the default exceptional value.".

cs:NullFlavor\#NI a cs:NullFlavor.class\#NI.

cs:NullFlavor.class\#INV rdfs:subClassOf cs:NullFlavor.class\#NI;
  owl:oneOf (cs:NullFlavor\#INV cs:NullFlavor\#DER cs:NullFlavor\#OTH cs:NullFlavor\#NINF cs:NullFlavor\#PINF cs:NullFlavor\#UNC);
  rdfs:label "invalid";
  dc:title "invalid";
  rdfs:comment "Description:The value as represented in the instance is not a member of the set of permitted data values in the constrained value domain of a variable.";
  dcterms:description "Description:The value as represented in the instance is not a member of the set of permitted data values in the constrained value domain of a variable.".

cs:NullFlavor\#INV a cs:NullFlavor.class\#INV.

cs:NullFlavor.class\#DER rdfs:subClassOf cs:NullFlavor.class\#INV;
  owl:oneOf (cs:NullFlavor\#DER);
  rdfs:label "derived";
  dc:title "derived";
  rdfs:comment "Description:An actual value may exist, but it must be derived from the provided information (usually an EXPR generic data type extension will be used to convey the derivation expressionexpression .";
  dcterms:description "Description:An actual value may exist, but it must be derived from the provided information (usually an EXPR generic data type extension will be used to convey the derivation expressionexpression .".

cs:NullFlavor\#DER a cs:NullFlavor.class\#DER.

cs:NullFlavor.class\#OTH rdfs:subClassOf cs:NullFlavor.class\#INV;
  owl:oneOf (cs:NullFlavor\#OTH cs:NullFlavor\#NINF cs:NullFlavor\#PINF);
  rdfs:label "other";
  dc:title "other";
  rdfs:comment "Description:The actual value is not a member of the set of permitted data values in the constrained value domain of a variable. (e.g., concept not provided by required code system).\r\n\n                        \n                           Usage Notes: This flavor and its specializations are most commonly used with the CD datatype and its flavors.  However, it may apply to *any* datatype where the constraints of the type are tighter than can be conveyed.  For example, a PQ that is for a true measured amount whose units are not supported in UCUM, a need to convey a REAL when the type has been constrained to INT, etc.\r\n\n                        With coded datatypes, this null flavor may only be used if the vocabulary binding has a coding strength of CNE.  By definition, all local codes and original text are part of the value set if the coding strength is CWE.";
  dcterms:description "Description:The actual value is not a member of the set of permitted data values in the constrained value domain of a variable. (e.g., concept not provided by required code system).\r\n\n                        \n                           Usage Notes: This flavor and its specializations are most commonly used with the CD datatype and its flavors.  However, it may apply to *any* datatype where the constraints of the type are tighter than can be conveyed.  For example, a PQ that is for a true measured amount whose units are not supported in UCUM, a need to convey a REAL when the type has been constrained to INT, etc.\r\n\n                        With coded datatypes, this null flavor may only be used if the vocabulary binding has a coding strength of CNE.  By definition, all local codes and original text are part of the value set if the coding strength is CWE.".

cs:NullFlavor\#OTH a cs:NullFlavor.class\#OTH.

cs:NullFlavor.class\#NINF rdfs:subClassOf cs:NullFlavor.class\#OTH;
  owl:oneOf (cs:NullFlavor\#NINF);
  rdfs:label "negative infinity";
  dc:title "negative infinity";
  rdfs:comment "Negative infinity of numbers.";
  dcterms:description "Negative infinity of numbers.".

cs:NullFlavor\#NINF a cs:NullFlavor.class\#NINF.

cs:NullFlavor.class\#PINF rdfs:subClassOf cs:NullFlavor.class\#OTH;
  owl:oneOf (cs:NullFlavor\#PINF);
  rdfs:label "positive infinity";
  dc:title "positive infinity";
  rdfs:comment "Positive infinity of numbers.";
  dcterms:description "Positive infinity of numbers.".

cs:NullFlavor\#PINF a cs:NullFlavor.class\#PINF.

cs:NullFlavor.class\#UNC rdfs:subClassOf cs:NullFlavor.class\#INV;
  owl:oneOf (cs:NullFlavor\#UNC);
  rdfs:label "un-encoded";
  dc:title "un-encoded";
  rdfs:comment "Description: The actual value has not yet been encoded within the approved value domain.\r\n\n                        \n                           Example: Original text or a local code has been specified but translation or encoding to the approved value set has not yet occurred due to limitations of the sending system.  Original text has been captured for a PQ, but not attempt has been made to split the value and unit or to encode the unit in UCUM.\r\n\n                        \n                           Usage Notes: If it is known that it is not possible to encode the concept, OTH should be used instead.  However, use of UNC does not necessarily guarantee the concept will be encodable, only that encoding has not been attempted.\r\n\n                        Data type properties such as original text and translations may be present when this null flavor is included.";
  dcterms:description "Description: The actual value has not yet been encoded within the approved value domain.\r\n\n                        \n                           Example: Original text or a local code has been specified but translation or encoding to the approved value set has not yet occurred due to limitations of the sending system.  Original text has been captured for a PQ, but not attempt has been made to split the value and unit or to encode the unit in UCUM.\r\n\n                        \n                           Usage Notes: If it is known that it is not possible to encode the concept, OTH should be used instead.  However, use of UNC does not necessarily guarantee the concept will be encodable, only that encoding has not been attempted.\r\n\n                        Data type properties such as original text and translations may be present when this null flavor is included.".

cs:NullFlavor\#UNC a cs:NullFlavor.class\#UNC.

cs:NullFlavor.class\#MSK rdfs:subClassOf cs:NullFlavor.class\#NI;
  owl:oneOf (cs:NullFlavor\#MSK);
  rdfs:label "masked";
  dc:title "masked";
  rdfs:comment "There is information on this item available but it has not been provided by the sender due to security, privacy or other reasons. There may be an alternate mechanism for gaining access to this information.\r\n\n                        Note: using this null flavor does provide information that may be a breach of confidentiality, even though no detail data is provided.  Its primary purpose is for those circumstances where it is necessary to inform the receiver that the information does exist without providing any detail.";
  dcterms:description "There is information on this item available but it has not been provided by the sender due to security, privacy or other reasons. There may be an alternate mechanism for gaining access to this information.\r\n\n                        Note: using this null flavor does provide information that may be a breach of confidentiality, even though no detail data is provided.  Its primary purpose is for those circumstances where it is necessary to inform the receiver that the information does exist without providing any detail.".

cs:NullFlavor\#MSK a cs:NullFlavor.class\#MSK.

cs:NullFlavor.class\#NA rdfs:subClassOf cs:NullFlavor.class\#NI;
  owl:oneOf (cs:NullFlavor\#NA);
  rdfs:label "not applicable";
  dc:title "not applicable";
  rdfs:comment "Known to have no proper value (e.g., last menstrual period for a male).";
  dcterms:description "Known to have no proper value (e.g., last menstrual period for a male).".

cs:NullFlavor\#NA a cs:NullFlavor.class\#NA.

cs:NullFlavor.class\#UNK rdfs:subClassOf cs:NullFlavor.class\#NI;
  owl:oneOf (cs:NullFlavor\#UNK cs:NullFlavor\#ASKU cs:NullFlavor\#NAV cs:NullFlavor\#NASK cs:NullFlavor\#QS cs:NullFlavor\#TRC);
  rdfs:label "unknown";
  dc:title "unknown";
  rdfs:comment "Description:A proper value is applicable, but not known.\r\n\n                        \n                           Usage Notes: This means the actual value is not known.  If the only thing that is unknown is how to properly express the value in the necessary constraints (value set, datatype, etc.), then the OTH or UNC flavor should be used.  No properties should be included for a datatype with this property unless:\r\n\n                        \n                           Those properties themselves directly translate to a semantic of \"unknown\".  (E.g. a local code sent as a translation that conveys 'unknown')\n                           Those properties further qualify the nature of what is unknown.  (E.g. specifying a use code of \"H\" and a URL prefix of \"tel:\" to convey that it is the home phone number that is unknown.)";
  dcterms:description "Description:A proper value is applicable, but not known.\r\n\n                        \n                           Usage Notes: This means the actual value is not known.  If the only thing that is unknown is how to properly express the value in the necessary constraints (value set, datatype, etc.), then the OTH or UNC flavor should be used.  No properties should be included for a datatype with this property unless:\r\n\n                        \n                           Those properties themselves directly translate to a semantic of \"unknown\".  (E.g. a local code sent as a translation that conveys 'unknown')\n                           Those properties further qualify the nature of what is unknown.  (E.g. specifying a use code of \"H\" and a URL prefix of \"tel:\" to convey that it is the home phone number that is unknown.)".

cs:NullFlavor\#UNK a cs:NullFlavor.class\#UNK.

cs:NullFlavor.class\#ASKU rdfs:subClassOf cs:NullFlavor.class\#UNK;
  owl:oneOf (cs:NullFlavor\#ASKU cs:NullFlavor\#NAV);
  rdfs:label "asked but unknown";
  dc:title "asked but unknown";
  rdfs:comment "Information was sought but not found (e.g., patient was asked but didn't know)";
  dcterms:description "Information was sought but not found (e.g., patient was asked but didn't know)".

cs:NullFlavor\#ASKU a cs:NullFlavor.class\#ASKU.

cs:NullFlavor.class\#NAV rdfs:subClassOf cs:NullFlavor.class\#ASKU;
  owl:oneOf (cs:NullFlavor\#NAV);
  rdfs:label "temporarily unavailable";
  dc:title "temporarily unavailable";
  rdfs:comment "Information is not available at this time but it is expected that it will be available later.";
  dcterms:description "Information is not available at this time but it is expected that it will be available later.".

cs:NullFlavor\#NAV a cs:NullFlavor.class\#NAV.

cs:NullFlavor.class\#NASK rdfs:subClassOf cs:NullFlavor.class\#UNK;
  owl:oneOf (cs:NullFlavor\#NASK);
  rdfs:label "not asked";
  dc:title "not asked";
  rdfs:comment "This information has not been sought (e.g., patient was not asked)";
  dcterms:description "This information has not been sought (e.g., patient was not asked)".

cs:NullFlavor\#NASK a cs:NullFlavor.class\#NASK.

cs:NullFlavor.class\#QS rdfs:subClassOf cs:NullFlavor.class\#UNK;
  owl:oneOf (cs:NullFlavor\#QS);
  rdfs:label "Sufficient Quantity";
  dc:title "Sufficient Quantity";
  rdfs:comment "Description:The specific quantity is not known, but is known to be non-zero and is not specified because it makes up the bulk of the material. e.g. 'Add 10mg of ingredient X, 50mg of ingredient Y, and sufficient quantity of water to 100mL.' The null flavor would be used to express the quantity of water.";
  dcterms:description "Description:The specific quantity is not known, but is known to be non-zero and is not specified because it makes up the bulk of the material. e.g. 'Add 10mg of ingredient X, 50mg of ingredient Y, and sufficient quantity of water to 100mL.' The null flavor would be used to express the quantity of water.".

cs:NullFlavor\#QS a cs:NullFlavor.class\#QS.

cs:NullFlavor.class\#TRC rdfs:subClassOf cs:NullFlavor.class\#UNK;
  owl:oneOf (cs:NullFlavor\#TRC);
  rdfs:label "trace";
  dc:title "trace";
  rdfs:comment "The content is greater than zero, but too small to be quantified.";
  dcterms:description "The content is greater than zero, but too small to be quantified.".

cs:NullFlavor\#TRC a cs:NullFlavor.class\#TRC.


# - vs:EntityClass -------------------------------------------------------------

vs:EntityClass a fhir:ValueSet;
  fhir:version "2015-03-23";
  rdfs:label "v3 Code System EntityClass";
  dc:title "v3 Code System EntityClass";
  rdfs:comment " Classifies the Entity class and all of its subclasses.  The terminology is hierarchical.  At the top is this  HL7-defined domain of high-level categories (such as represented by the Entity subclasses). Each of these terms must be harmonized and is specializable. The value sets beneath are drawn from multiple, frequently external, domains that reflect much more fine-grained typing.";
  dcterms:description " Classifies the Entity class and all of its subclasses.  The terminology is hierarchical.  At the top is this  HL7-defined domain of high-level categories (such as represented by the Entity subclasses). Each of these terms must be harmonized and is specializable. The value sets beneath are drawn from multiple, frequently external, domains that reflect much more fine-grained typing.";
  dc:date "Mon Mar 23 00:00:00 EST 2015";
  fhir:status fhir:conformance-resource-status\#active;
  fhir:canonical-status fhir:canonical-status-codes\#active;
  fhir:include cs:EntityClass.

cs:EntityClass a fhir:CodeSystem;
  rdfs:label "v3 Code System EntityClass";
  dc:title "v3 Code System EntityClass";
  rdfs:comment " Classifies the Entity class and all of its subclasses.  The terminology is hierarchical.  At the top is this  HL7-defined domain of high-level categories (such as represented by the Entity subclasses). Each of these terms must be harmonized and is specializable. The code systems beneath are drawn from multiple, frequently external, domains that reflect much more fine-grained typing.";
  dcterms:description " Classifies the Entity class and all of its subclasses.  The terminology is hierarchical.  At the top is this  HL7-defined domain of high-level categories (such as represented by the Entity subclasses). Each of these terms must be harmonized and is specializable. The code systems beneath are drawn from multiple, frequently external, domains that reflect much more fine-grained typing.";
  dc:date "Mon Mar 23 00:00:00 EST 2015";
  fhir:concepts cs:EntityClass.class.

cs:EntityClass.class a fhir:Concept;
  owl:oneOf (cs:EntityClass\#ENT cs:EntityClass\#HCE cs:EntityClass\#LIV cs:EntityClass\#NLIV cs:EntityClass\#ANM cs:EntityClass\#MIC cs:EntityClass\#PLNT cs:EntityClass\#PSN cs:EntityClass\#MAT cs:EntityClass\#CHEM cs:EntityClass\#FOOD cs:EntityClass\#MMAT cs:EntityClass\#CONT cs:EntityClass\#HOLD cs:EntityClass\#DEV cs:EntityClass\#CER cs:EntityClass\#MODDV cs:EntityClass\#ORG cs:EntityClass\#PUB cs:EntityClass\#STATE cs:EntityClass\#NAT cs:EntityClass\#PLC cs:EntityClass\#CITY cs:EntityClass\#COUNTRY cs:EntityClass\#COUNTY cs:EntityClass\#PROVINCE cs:EntityClass\#RGRP).

cs:EntityClass.class\#ENT rdfs:subClassOf cs:EntityClass.class;
  owl:oneOf (cs:EntityClass\#ENT cs:EntityClass\#HCE cs:EntityClass\#LIV cs:EntityClass\#NLIV cs:EntityClass\#ANM cs:EntityClass\#MIC cs:EntityClass\#PLNT cs:EntityClass\#PSN cs:EntityClass\#MAT cs:EntityClass\#CHEM cs:EntityClass\#FOOD cs:EntityClass\#MMAT cs:EntityClass\#CONT cs:EntityClass\#HOLD cs:EntityClass\#DEV cs:EntityClass\#CER cs:EntityClass\#MODDV cs:EntityClass\#ORG cs:EntityClass\#PUB cs:EntityClass\#STATE cs:EntityClass\#NAT cs:EntityClass\#PLC cs:EntityClass\#CITY cs:EntityClass\#COUNTRY cs:EntityClass\#COUNTY cs:EntityClass\#PROVINCE cs:EntityClass\#RGRP);
  rdfs:label "entity";
  dc:title "entity";
  rdfs:comment "Corresponds to the Entity class";
  dcterms:description "Corresponds to the Entity class".

cs:EntityClass\#ENT a cs:EntityClass.class\#ENT.

cs:EntityClass.class\#HCE rdfs:subClassOf cs:EntityClass.class\#ENT;
  owl:oneOf (cs:EntityClass\#HCE);
  rdfs:label "health chart entity";
  dc:title "health chart entity";
  rdfs:comment "A health chart included to serve as a document receiving entity in the management of medical records.";
  dcterms:description "A health chart included to serve as a document receiving entity in the management of medical records.".

cs:EntityClass\#HCE a cs:EntityClass.class\#HCE.

cs:EntityClass.class\#LIV rdfs:subClassOf cs:EntityClass.class\#ENT;
  owl:oneOf (cs:EntityClass\#LIV cs:EntityClass\#NLIV cs:EntityClass\#ANM cs:EntityClass\#MIC cs:EntityClass\#PLNT cs:EntityClass\#PSN);
  rdfs:label "living subject";
  dc:title "living subject";
  rdfs:comment "Anything that essentially has the property of life, independent of current state (a dead human corpse is still essentially a living subject).";
  dcterms:description "Anything that essentially has the property of life, independent of current state (a dead human corpse is still essentially a living subject).".

cs:EntityClass\#LIV a cs:EntityClass.class\#LIV.

cs:EntityClass.class\#NLIV rdfs:subClassOf cs:EntityClass.class\#LIV;
  owl:oneOf (cs:EntityClass\#NLIV cs:EntityClass\#ANM cs:EntityClass\#MIC cs:EntityClass\#PLNT);
  rdfs:label "non-person living subject";
  dc:title "non-person living subject";
  rdfs:comment "A subtype of living subject that includes all living things except the species Homo Sapiens.";
  dcterms:description "A subtype of living subject that includes all living things except the species Homo Sapiens.".

cs:EntityClass\#NLIV a cs:EntityClass.class\#NLIV.

cs:EntityClass.class\#ANM rdfs:subClassOf cs:EntityClass.class\#NLIV;
  owl:oneOf (cs:EntityClass\#ANM);
  rdfs:label "animal";
  dc:title "animal";
  rdfs:comment "A living subject from the animal kingdom.";
  dcterms:description "A living subject from the animal kingdom.".

cs:EntityClass\#ANM a cs:EntityClass.class\#ANM.

cs:EntityClass.class\#MIC rdfs:subClassOf cs:EntityClass.class\#NLIV;
  owl:oneOf (cs:EntityClass\#MIC);
  rdfs:label "microorganism";
  dc:title "microorganism";
  rdfs:comment "All single celled living organisms including protozoa, bacteria, yeast, viruses, etc.";
  dcterms:description "All single celled living organisms including protozoa, bacteria, yeast, viruses, etc.".

cs:EntityClass\#MIC a cs:EntityClass.class\#MIC.

cs:EntityClass.class\#PLNT rdfs:subClassOf cs:EntityClass.class\#NLIV;
  owl:oneOf (cs:EntityClass\#PLNT);
  rdfs:label "plant";
  dc:title "plant";
  rdfs:comment "A living subject from the order of plants.";
  dcterms:description "A living subject from the order of plants.".

cs:EntityClass\#PLNT a cs:EntityClass.class\#PLNT.

cs:EntityClass.class\#PSN rdfs:subClassOf cs:EntityClass.class\#LIV;
  owl:oneOf (cs:EntityClass\#PSN);
  rdfs:label "person";
  dc:title "person";
  rdfs:comment "A living subject of the species homo sapiens.";
  dcterms:description "A living subject of the species homo sapiens.".

cs:EntityClass\#PSN a cs:EntityClass.class\#PSN.

cs:EntityClass.class\#MAT rdfs:subClassOf cs:EntityClass.class\#ENT;
  owl:oneOf (cs:EntityClass\#MAT cs:EntityClass\#CHEM cs:EntityClass\#FOOD cs:EntityClass\#MMAT cs:EntityClass\#CONT cs:EntityClass\#HOLD cs:EntityClass\#DEV cs:EntityClass\#CER cs:EntityClass\#MODDV);
  rdfs:label "material";
  dc:title "material";
  rdfs:comment "Any thing that has extension in space and mass, may be of living or non-living origin.";
  dcterms:description "Any thing that has extension in space and mass, may be of living or non-living origin.".

cs:EntityClass\#MAT a cs:EntityClass.class\#MAT.

cs:EntityClass.class\#CHEM rdfs:subClassOf cs:EntityClass.class\#MAT;
  owl:oneOf (cs:EntityClass\#CHEM);
  rdfs:label "chemical substance";
  dc:title "chemical substance";
  rdfs:comment "A substance that is fully defined by an organic or inorganic chemical formula, includes mixtures of other chemical substances. Refine using, e.g., IUPAC codes.";
  dcterms:description "A substance that is fully defined by an organic or inorganic chemical formula, includes mixtures of other chemical substances. Refine using, e.g., IUPAC codes.".

cs:EntityClass\#CHEM a cs:EntityClass.class\#CHEM.

cs:EntityClass.class\#FOOD rdfs:subClassOf cs:EntityClass.class\#MAT;
  owl:oneOf (cs:EntityClass\#FOOD);
  rdfs:label "food";
  dc:title "food";
  rdfs:comment "Naturally occurring, processed or manufactured entities that are primarily used as food for humans and animals.";
  dcterms:description "Naturally occurring, processed or manufactured entities that are primarily used as food for humans and animals.".

cs:EntityClass\#FOOD a cs:EntityClass.class\#FOOD.

cs:EntityClass.class\#MMAT rdfs:subClassOf cs:EntityClass.class\#MAT;
  owl:oneOf (cs:EntityClass\#MMAT cs:EntityClass\#CONT cs:EntityClass\#HOLD cs:EntityClass\#DEV cs:EntityClass\#CER cs:EntityClass\#MODDV);
  rdfs:label "manufactured material";
  dc:title "manufactured material";
  rdfs:comment "Corresponds to the ManufacturedMaterial class";
  dcterms:description "Corresponds to the ManufacturedMaterial class".

cs:EntityClass\#MMAT a cs:EntityClass.class\#MMAT.

cs:EntityClass.class\#CONT rdfs:subClassOf cs:EntityClass.class\#MMAT;
  owl:oneOf (cs:EntityClass\#CONT cs:EntityClass\#HOLD);
  rdfs:label "container";
  dc:title "container";
  rdfs:comment "A container of other entities.";
  dcterms:description "A container of other entities.".

cs:EntityClass\#CONT a cs:EntityClass.class\#CONT.

cs:EntityClass.class\#HOLD rdfs:subClassOf cs:EntityClass.class\#CONT;
  owl:oneOf (cs:EntityClass\#HOLD);
  rdfs:label "holder";
  dc:title "holder";
  rdfs:comment "A type of container that can hold other containers or other holders.";
  dcterms:description "A type of container that can hold other containers or other holders.".

cs:EntityClass\#HOLD a cs:EntityClass.class\#HOLD.

cs:EntityClass.class\#DEV rdfs:subClassOf cs:EntityClass.class\#MMAT;
  owl:oneOf (cs:EntityClass\#DEV cs:EntityClass\#CER cs:EntityClass\#MODDV);
  rdfs:label "device";
  dc:title "device";
  rdfs:comment "A subtype of ManufacturedMaterial used in an activity, without being substantially changed through that activity.  The kind of device is identified by the code attribute inherited from Entity.\r\n\n                        \n                           Usage: This includes durable (reusable) medical equipment as well as disposable equipment.";
  dcterms:description "A subtype of ManufacturedMaterial used in an activity, without being substantially changed through that activity.  The kind of device is identified by the code attribute inherited from Entity.\r\n\n                        \n                           Usage: This includes durable (reusable) medical equipment as well as disposable equipment.".

cs:EntityClass\#DEV a cs:EntityClass.class\#DEV.

cs:EntityClass.class\#CER rdfs:subClassOf cs:EntityClass.class\#DEV;
  owl:oneOf (cs:EntityClass\#CER);
  rdfs:label "certificate representation";
  dc:title "certificate representation";
  rdfs:comment "A physical artifact that stores information about the granting of authorization.";
  dcterms:description "A physical artifact that stores information about the granting of authorization.".

cs:EntityClass\#CER a cs:EntityClass.class\#CER.

cs:EntityClass.class\#MODDV rdfs:subClassOf cs:EntityClass.class\#DEV;
  owl:oneOf (cs:EntityClass\#MODDV);
  rdfs:label "imaging modality";
  dc:title "imaging modality";
  rdfs:comment "Class to contain unique attributes of diagnostic imaging equipment.";
  dcterms:description "Class to contain unique attributes of diagnostic imaging equipment.".

cs:EntityClass\#MODDV a cs:EntityClass.class\#MODDV.

cs:EntityClass.class\#ORG rdfs:subClassOf cs:EntityClass.class\#ENT;
  owl:oneOf (cs:EntityClass\#ORG cs:EntityClass\#PUB cs:EntityClass\#STATE cs:EntityClass\#NAT);
  rdfs:label "organization";
  dc:title "organization";
  rdfs:comment "A social or legal structure formed by human beings.";
  dcterms:description "A social or legal structure formed by human beings.".

cs:EntityClass\#ORG a cs:EntityClass.class\#ORG.

cs:EntityClass.class\#PUB rdfs:subClassOf cs:EntityClass.class\#ORG;
  owl:oneOf (cs:EntityClass\#PUB);
  rdfs:label "public institution";
  dc:title "public institution";
  rdfs:comment "An agency of the people of a state often assuming some authority over a certain matter. Includes government, governmental agencies, associations.";
  dcterms:description "An agency of the people of a state often assuming some authority over a certain matter. Includes government, governmental agencies, associations.".

cs:EntityClass\#PUB a cs:EntityClass.class\#PUB.

cs:EntityClass.class\#STATE rdfs:subClassOf cs:EntityClass.class\#ORG;
  owl:oneOf (cs:EntityClass\#STATE cs:EntityClass\#NAT);
  rdfs:label "state";
  dc:title "state";
  rdfs:comment "A politically organized body of people bonded by territory, culture, or ethnicity, having sovereignty (to a certain extent) granted by other states (enclosing or neighboring states). This includes countries (nations), provinces (e.g., one of the United States of America or a French departement), counties or municipalities. Refine using, e.g., ISO country codes, FIPS-PUB state codes, etc.";
  dcterms:description "A politically organized body of people bonded by territory, culture, or ethnicity, having sovereignty (to a certain extent) granted by other states (enclosing or neighboring states). This includes countries (nations), provinces (e.g., one of the United States of America or a French departement), counties or municipalities. Refine using, e.g., ISO country codes, FIPS-PUB state codes, etc.".

cs:EntityClass\#STATE a cs:EntityClass.class\#STATE.

cs:EntityClass.class\#NAT rdfs:subClassOf cs:EntityClass.class\#STATE;
  owl:oneOf (cs:EntityClass\#NAT);
  rdfs:label "Nation";
  dc:title "Nation";
  rdfs:comment "A politically organized body of people bonded by territory and known as a nation.";
  dcterms:description "A politically organized body of people bonded by territory and known as a nation.".

cs:EntityClass\#NAT a cs:EntityClass.class\#NAT.

cs:EntityClass.class\#PLC rdfs:subClassOf cs:EntityClass.class\#ENT;
  owl:oneOf (cs:EntityClass\#PLC cs:EntityClass\#CITY cs:EntityClass\#COUNTRY cs:EntityClass\#COUNTY cs:EntityClass\#PROVINCE);
  rdfs:label "place";
  dc:title "place";
  rdfs:comment "A physical place or site with its containing structure. May be natural or man-made. The geographic position of a place may or may not be constant.";
  dcterms:description "A physical place or site with its containing structure. May be natural or man-made. The geographic position of a place may or may not be constant.".

cs:EntityClass\#PLC a cs:EntityClass.class\#PLC.

cs:EntityClass.class\#CITY rdfs:subClassOf cs:EntityClass.class\#PLC;
  owl:oneOf (cs:EntityClass\#CITY);
  rdfs:label "city or town";
  dc:title "city or town";
  rdfs:comment "The territory of a city, town or other municipality.";
  dcterms:description "The territory of a city, town or other municipality.".

cs:EntityClass\#CITY a cs:EntityClass.class\#CITY.

cs:EntityClass.class\#COUNTRY rdfs:subClassOf cs:EntityClass.class\#PLC;
  owl:oneOf (cs:EntityClass\#COUNTRY);
  rdfs:label "country";
  dc:title "country";
  rdfs:comment "The territory of a sovereign nation.";
  dcterms:description "The territory of a sovereign nation.".

cs:EntityClass\#COUNTRY a cs:EntityClass.class\#COUNTRY.

cs:EntityClass.class\#COUNTY rdfs:subClassOf cs:EntityClass.class\#PLC;
  owl:oneOf (cs:EntityClass\#COUNTY);
  rdfs:label "county or parish";
  dc:title "county or parish";
  rdfs:comment "The territory of a county, parish or other division of a state or province.";
  dcterms:description "The territory of a county, parish or other division of a state or province.".

cs:EntityClass\#COUNTY a cs:EntityClass.class\#COUNTY.

cs:EntityClass.class\#PROVINCE rdfs:subClassOf cs:EntityClass.class\#PLC;
  owl:oneOf (cs:EntityClass\#PROVINCE);
  rdfs:label "state or province";
  dc:title "state or province";
  rdfs:comment "The territory of a state, province, department or other division of a sovereign country.";
  dcterms:description "The territory of a state, province, department or other division of a sovereign country.".

cs:EntityClass\#PROVINCE a cs:EntityClass.class\#PROVINCE.

cs:EntityClass.class\#RGRP rdfs:subClassOf cs:EntityClass.class\#ENT;
  owl:oneOf (cs:EntityClass\#RGRP);
  rdfs:label "group";
  dc:title "group";
  rdfs:comment "A grouping of resources (personnel, material, or places) to be used for scheduling purposes.  May be a pool of like-type resources, a team, or combination of personnel, material and places.";
  dcterms:description "A grouping of resources (personnel, material, or places) to be used for scheduling purposes.  May be a pool of like-type resources, a team, or combination of personnel, material and places.".

cs:EntityClass\#RGRP a cs:EntityClass.class\#RGRP.

# - vs:EntityDeterminer --------------------------------------------------------

vs:EntityDeterminer a fhir:ValueSet;
  fhir:version "2015-03-23";
  rdfs:label "v3 Code System EntityDeterminer";
  dc:title "v3 Code System EntityDeterminer";
  rdfs:comment " EntityDeterminer in natural language grammar is the class of words that comprises articles, demonstrative pronouns, and quantifiers. In the RIM, determiner is a structural code in the Entity class to distinguish whether any given Entity object stands for some, any one, or a specific thing.";
  dcterms:description " EntityDeterminer in natural language grammar is the class of words that comprises articles, demonstrative pronouns, and quantifiers. In the RIM, determiner is a structural code in the Entity class to distinguish whether any given Entity object stands for some, any one, or a specific thing.";
  dc:date "2015-03-23";
  fhir:status fhir:conformance-resource-status\#active;
  fhir:canonical-status fhir:canonical-status-codes\#active;
  fhir:include cs:EntityDeterminer.

cs:EntityDeterminer a fhir:CodeSystem;
  rdfs:label "v3 Code System EntityDeterminer";
  dc:title "v3 Code System EntityDeterminer";
  rdfs:comment " EntityDeterminer in natural language grammar is the class of words that comprises articles, demonstrative pronouns, and quantifiers. In the RIM, determiner is a structural code in the Entity class to distinguish whether any given Entity object stands for some, any one, or a specific thing.";
  dcterms:description " EntityDeterminer in natural language grammar is the class of words that comprises articles, demonstrative pronouns, and quantifiers. In the RIM, determiner is a structural code in the Entity class to distinguish whether any given Entity object stands for some, any one, or a specific thing.";
  dc:date "Mon Mar 23 00:00:00 EST 2015".

cs:EntityDeterminer.class a fhir:Concept;
  owl:oneOf (cs:EntityDeterminer\#INSTANCE cs:EntityDeterminer\#GROUP cs:EntityDeterminer\#KIND cs:EntityDeterminer\#GROUPKIND).

cs:EntityDeterminer.class\#INSTANCE rdfs:subClassOf cs:EntityDeterminer.class;
  owl:oneOf (cs:EntityDeterminer\#INSTANCE cs:EntityDeterminer\#GROUP);
  rdfs:label "specific";
  dc:title "specific";
  rdfs:comment "Description:A determiner that specifies that the Entity object represents a particular physical thing (as opposed to a universal, kind, or class of physical thing).\r\n\n                        \n                           Discussion: It does not matter whether an INSTANCE still exists as a whole at the point in time (or process) when we mention it, for example, a drug product lot is an INSTANCE even though it has been portioned out for retail purpose.";
  dcterms:description "Description:A determiner that specifies that the Entity object represents a particular physical thing (as opposed to a universal, kind, or class of physical thing).\r\n\n                        \n                           Discussion: It does not matter whether an INSTANCE still exists as a whole at the point in time (or process) when we mention it, for example, a drug product lot is an INSTANCE even though it has been portioned out for retail purpose.".

cs:EntityDeterminer\#INSTANCE a cs:EntityDeterminer.class\#INSTANCE.

cs:EntityDeterminer.class\#GROUP rdfs:subClassOf cs:EntityDeterminer.class\#INSTANCE;
  owl:oneOf (cs:EntityDeterminer\#GROUP);
  rdfs:label "specific group";
  dc:title "specific group";
  rdfs:comment "A determiner that specifies that the Entity object represents a particular collection of physical things (as opposed to a universal, kind, or class of physical thing).  While the collection may resolve to having only a single individual (or even no individuals), the potential should exist for it to cover multiple individuals.";
  dcterms:description "A determiner that specifies that the Entity object represents a particular collection of physical things (as opposed to a universal, kind, or class of physical thing).  While the collection may resolve to having only a single individual (or even no individuals), the potential should exist for it to cover multiple individuals.".

cs:EntityDeterminer\#GROUP a cs:EntityDeterminer.class\#GROUP.

cs:EntityDeterminer.class\#KIND rdfs:subClassOf cs:EntityDeterminer.class;
  owl:oneOf (cs:EntityDeterminer\#KIND cs:EntityDeterminer\#GROUPKIND);
  rdfs:label "described";
  dc:title "described";
  rdfs:comment "Description:A determiner that specifies that the Entity object represents a universal, kind or class of physical thing (as opposed to a particular thing).";
  dcterms:description "Description:A determiner that specifies that the Entity object represents a universal, kind or class of physical thing (as opposed to a particular thing).".

cs:EntityDeterminer\#KIND a cs:EntityDeterminer.class\#KIND.

cs:EntityDeterminer.class\#GROUPKIND rdfs:subClassOf cs:EntityDeterminer.class\#KIND;
  owl:oneOf (cs:EntityDeterminer\#GROUPKIND);
  rdfs:label "described group";
  dc:title "described group";
  rdfs:comment "A determiner that specifies that the Entity object represents a universal, kind or class of collections physical things.  While the collection may resolve to having only a single individual (or even no individuals), the potential should exist for it to cover multiple individuals.";
  dcterms:description "A determiner that specifies that the Entity object represents a universal, kind or class of collections physical things.  While the collection may resolve to having only a single individual (or even no individuals), the potential should exist for it to cover multiple individuals.".

cs:EntityDeterminer\#GROUPKIND a cs:EntityDeterminer.class\#GROUPKIND.

# - vs:EntityStatus ------------------------------------------------------------

vs:EntityStatus a fhir:ValueSet;
  fhir:version "2015-03-23";
  rdfs:label "v3 Code System EntityStatus";
  dc:title "v3 Code System EntityStatus";
  rdfs:comment " Codes representing the defined possible states of an Entity, as defined by the Entity class state machine.";
  dcterms:description " Codes representing the defined possible states of an Entity, as defined by the Entity class state machine.";
  dc:date "2015-03-23";
  fhir:status fhir:conformance-resource-status\#active;
  fhir:canonical-status fhir:canonical-status-codes\#active;
  fhir:include cs:EntityStatus.

cs:EntityStatus a fhir:CodeSystem;
  rdfs:label "v3 Code System EntityStatus";
  dc:title "v3 Code System EntityStatus";
  rdfs:comment " Codes representing the defined possible states of an Entity, as defined by the Entity class state machine.";
  dcterms:description " Codes representing the defined possible states of an Entity, as defined by the Entity class state machine.";
  dc:date "Mon Mar 23 00:00:00 EST 2015".

cs:EntityStatus.class a fhir:Concept;
  owl:oneOf (cs:EntityStatus\#normal cs:EntityStatus\#active cs:EntityStatus\#inactive cs:EntityStatus\#nullified).

cs:EntityStatus.class\#normal rdfs:subClassOf cs:EntityStatus.class;
  owl:oneOf (cs:EntityStatus\#normal cs:EntityStatus\#active cs:EntityStatus\#inactive);
  rdfs:label "normal";
  dc:title "normal";
  rdfs:comment "The 'typical' state. Excludes \"nullified\" which represents the termination state of an Entity record instance that was created in error.";
  dcterms:description "The 'typical' state. Excludes \"nullified\" which represents the termination state of an Entity record instance that was created in error.".

cs:EntityStatus\#normal a cs:EntityStatus.class\#normal.

cs:EntityStatus.class\#active rdfs:subClassOf cs:EntityStatus.class\#normal;
  owl:oneOf (cs:EntityStatus\#active);
  rdfs:label "active";
  dc:title "active";
  rdfs:comment "The state representing the fact that the Entity record is currently active.";
  dcterms:description "The state representing the fact that the Entity record is currently active.".

cs:EntityStatus\#active a cs:EntityStatus.class\#active.

cs:EntityStatus.class\#inactive rdfs:subClassOf cs:EntityStatus.class\#normal;
  owl:oneOf (cs:EntityStatus\#inactive);
  rdfs:label "inactive";
  dc:title "inactive";
  rdfs:comment "Definition: The state representing the fact that the entity is inactive.";
  dcterms:description "Definition: The state representing the fact that the entity is inactive.".

cs:EntityStatus\#inactive a cs:EntityStatus.class\#inactive.

cs:EntityStatus.class\#nullified rdfs:subClassOf cs:EntityStatus.class;
  owl:oneOf (cs:EntityStatus\#nullified);
  rdfs:label "nullified";
  dc:title "nullified";
  rdfs:comment "The state representing the termination of an Entity record instance that was created in error.";
  dcterms:description "The state representing the termination of an Entity record instance that was created in error.".

cs:EntityStatus\#nullified a cs:EntityStatus.class\#nullified.

# - vs:IdentifierScope ---------------------------------------------------------

vs:IdentifierScope a fhir:ValueSet;
  fhir:version "2015-03-23";
  rdfs:label "v3 Code System IdentifierScope";
  dc:title "v3 Code System IdentifierScope";
  rdfs:comment "  Description:\r\nCodes to specify the scope in which the identifier applies to the object with which it is associated, and used in the datatype property II.";
  dcterms:description "  Description:\r\nCodes to specify the scope in which the identifier applies to the object with which it is associated, and used in the datatype property II.";
  dc:date "2015-03-23";
  fhir:status fhir:conformance-resource-status\#active;
  fhir:canonical-status fhir:canonical-status-codes\#active;
  fhir:include cs:IdentifierScope.

cs:IdentifierScope a fhir:CodeSystem;
  rdfs:label "v3 Code System IdentifierScope";
  dc:title "v3 Code System IdentifierScope";
  rdfs:comment "  Description:\r\nCodes to specify the scope in which the identifier applies to the object with which it is associated, and used in the datatype property II.";
  dcterms:description "  Description:\r\nCodes to specify the scope in which the identifier applies to the object with which it is associated, and used in the datatype property II.";
  dc:date "Mon Mar 23 00:00:00 EST 2015".

cs:IdentifierScope.class a fhir:Concept;
  owl:oneOf (cs:IdentifierScope\#BUSN cs:IdentifierScope\#OBJ cs:IdentifierScope\#VER cs:IdentifierScope\#VW).

cs:IdentifierScope.class\#BUSN rdfs:subClassOf cs:IdentifierScope.class;
  owl:oneOf (cs:IdentifierScope\#BUSN);
  rdfs:label "Business Identifier";
  dc:title "Business Identifier";
  rdfs:comment "Description: An identifier whose scope is defined by the business practices associated with the object. In contrast to the other scope identifiers, the scope of the use of the id is not necessarily restricted to a single object, but may be reused for other objects closely associated with the object due to business practice.";
  dcterms:description "Description: An identifier whose scope is defined by the business practices associated with the object. In contrast to the other scope identifiers, the scope of the use of the id is not necessarily restricted to a single object, but may be reused for other objects closely associated with the object due to business practice.".

cs:IdentifierScope\#BUSN a cs:IdentifierScope.class\#BUSN.

cs:IdentifierScope.class\#OBJ rdfs:subClassOf cs:IdentifierScope.class;
  owl:oneOf (cs:IdentifierScope\#OBJ);
  rdfs:label "Object Identifier";
  dc:title "Object Identifier";
  rdfs:comment "Description: The identifier associated with a particular object. It remains consistent as the object undergoes state transitions.";
  dcterms:description "Description: The identifier associated with a particular object. It remains consistent as the object undergoes state transitions.".

cs:IdentifierScope\#OBJ a cs:IdentifierScope.class\#OBJ.

cs:IdentifierScope.class\#VER rdfs:subClassOf cs:IdentifierScope.class;
  owl:oneOf (cs:IdentifierScope\#VER);
  rdfs:label "Version Identifier";
  dc:title "Version Identifier";
  rdfs:comment "Description: An identifier that references a particular object as it existed at a given point in time. The identifier SHALL change with each state transition on the object. I.e. The version identifier of an object prior to a 'suspend' state transition is distinct from the identifier of the object after the state transition. Each version identifier can be tied to exactly one ControlAct event which brought that version into being (though the control act may never be instantiated).\r\n\n                        \n                            NOTE: Applications that do not support versioning of objects must ignore and not persist these ids to avoid confusion resulting from leaving the same identifier on an object that undergoes changes.";
  dcterms:description "Description: An identifier that references a particular object as it existed at a given point in time. The identifier SHALL change with each state transition on the object. I.e. The version identifier of an object prior to a 'suspend' state transition is distinct from the identifier of the object after the state transition. Each version identifier can be tied to exactly one ControlAct event which brought that version into being (though the control act may never be instantiated).\r\n\n                        \n                            NOTE: Applications that do not support versioning of objects must ignore and not persist these ids to avoid confusion resulting from leaving the same identifier on an object that undergoes changes.".

cs:IdentifierScope\#VER a cs:IdentifierScope.class\#VER.

cs:IdentifierScope.class\#VW rdfs:subClassOf cs:IdentifierScope.class;
  owl:oneOf (cs:IdentifierScope\#VW);
  rdfs:label "View Specific Identifier";
  dc:title "View Specific Identifier";
  rdfs:comment "Description: An identifier that references a particular object as it existed at a given point in time. The identifier SHALL change with each state transition on the object.\r\n\n                        \n                           Example The version identifier of an object prior to a 'suspend' state transition is distinct from the identifier of the object after the state transition. Each version identifier can be tied to exactly one ControlAct event which brought that version into being (though the control act may never be instantiated).\r\n\n                        \n                            NOTE: Applications that do not support versioning of objects must ignore and not persist these ids to avoid confusion resulting from leaving the same identifier on an object that undergoes changes.";
  dcterms:description "Description: An identifier that references a particular object as it existed at a given point in time. The identifier SHALL change with each state transition on the object.\r\n\n                        \n                           Example The version identifier of an object prior to a 'suspend' state transition is distinct from the identifier of the object after the state transition. Each version identifier can be tied to exactly one ControlAct event which brought that version into being (though the control act may never be instantiated).\r\n\n                        \n                            NOTE: Applications that do not support versioning of objects must ignore and not persist these ids to avoid confusion resulting from leaving the same identifier on an object that undergoes changes.".

cs:IdentifierScope\#VW a cs:IdentifierScope.class\#VW.

# - vs:IdentifierReliability ---------------------------------------------------

vs:IdentifierReliability a fhir:ValueSet;
  fhir:version "2015-03-23";
  rdfs:label "v3 Code System IdentifierReliability";
  dc:title "v3 Code System IdentifierReliability";
  rdfs:comment " Specifies the reliability with which the identifier is known. This attribute MAY be used to assist with identifier matching algorithms.";
  dcterms:description " Specifies the reliability with which the identifier is known. This attribute MAY be used to assist with identifier matching algorithms.";
  dc:date "2015-03-23";
  fhir:status fhir:conformance-resource-status\#active;
  fhir:canonical-status fhir:canonical-status-codes\#active;
  fhir:include cs:IdentifierReliability.

cs:IdentifierReliability a fhir:CodeSystem;
  rdfs:label "v3 Code System IdentifierReliability";
  dc:title "v3 Code System IdentifierReliability";
  rdfs:comment " Specifies the reliability with which the identifier is known. This attribute MAY be used to assist with identifier matching algorithms.";
  dcterms:description " Specifies the reliability with which the identifier is known. This attribute MAY be used to assist with identifier matching algorithms.";
  dc:date "Mon Mar 23 00:00:00 EST 2015".

cs:IdentifierReliability.class a fhir:Concept;
  owl:oneOf (cs:IdentifierReliability\#ISS cs:IdentifierReliability\#UNV cs:IdentifierReliability\#VRF).

cs:IdentifierReliability.class\#ISS rdfs:subClassOf cs:IdentifierReliability.class;
  owl:oneOf (cs:IdentifierReliability\#ISS);
  rdfs:label "Issued by System";
  dc:title "Issued by System";
  rdfs:comment "Description: The identifier was issued by the system responsible for constructing the instance.";
  dcterms:description "Description: The identifier was issued by the system responsible for constructing the instance.".

cs:IdentifierReliability\#ISS a cs:IdentifierReliability.class\#ISS.

cs:IdentifierReliability.class\#UNV rdfs:subClassOf cs:IdentifierReliability.class;
  owl:oneOf (cs:IdentifierReliability\#UNV);
  rdfs:label "Unverified by system";
  dc:title "Unverified by system";
  rdfs:comment "Description: The identifier was provided to the system that constructed the instance, but has not been verified. e.g. a Drivers  license entered manually into a system by a user.";
  dcterms:description "Description: The identifier was provided to the system that constructed the instance, but has not been verified. e.g. a Drivers  license entered manually into a system by a user.".

cs:IdentifierReliability\#UNV a cs:IdentifierReliability.class\#UNV.

cs:IdentifierReliability.class\#VRF rdfs:subClassOf cs:IdentifierReliability.class;
  owl:oneOf (cs:IdentifierReliability\#VRF);
  rdfs:label "Verified by system";
  dc:title "Verified by system";
  rdfs:comment "Description: The identifier was not issued by the system responsible for constructing the instance, but the system that captured the id has verified the identifier with the issuing authority, or with another system that has verified the identifier.";
  dcterms:description "Description: The identifier was not issued by the system responsible for constructing the instance, but the system that captured the id has verified the identifier with the issuing authority, or with another system that has verified the identifier.".

cs:IdentifierReliability\#VRF a cs:IdentifierReliability.class\#VRF.

# - vs:CodingRationale ---------------------------------------------------------

vs:CodingRationale a fhir:ValueSet;
  fhir:version "2015-03-23";
  rdfs:label "v3 Code System CodingRationale";
  dc:title "v3 Code System CodingRationale";
  rdfs:comment " Identifies how to interpret the instance of the code, codeSystem value in a set of translations.  Since HL7 (or a government body) may mandate that codes from certain value sets be sent in conformant messages, other synonyms that are sent in the translation set need to be distinguished among the originally captured source, the HL7 specified code, or some future role.  When this code is NULL, it indicates that the translation is an undefined type.  When valued, this property must contain one of the following values: SRC - Source (or original) code HL7 - HL7 Specified or Mandated SH - both HL7 mandated and the original code (precoordination) There may be additional values added to this value set as we work through the use of codes in messages and determine other Use Cases requiring special interpretation of the translations.";
  dcterms:description " Identifies how to interpret the instance of the code, codeSystem value in a set of translations.  Since HL7 (or a government body) may mandate that codes from certain value sets be sent in conformant messages, other synonyms that are sent in the translation set need to be distinguished among the originally captured source, the HL7 specified code, or some future role.  When this code is NULL, it indicates that the translation is an undefined type.  When valued, this property must contain one of the following values: SRC - Source (or original) code HL7 - HL7 Specified or Mandated SH - both HL7 mandated and the original code (precoordination) There may be additional values added to this value set as we work through the use of codes in messages and determine other Use Cases requiring special interpretation of the translations.";
  dc:date "2015-03-23";
  fhir:status fhir:conformance-resource-status\#active;
  fhir:canonical-status fhir:canonical-status-codes\#active;
  fhir:include cs:CodingRationale.

cs:CodingRationale a fhir:CodeSystem;
  rdfs:label "v3 Code System CodingRationale";
  dc:title "v3 Code System CodingRationale";
  rdfs:comment " Identifies how to interpret the instance of the code, codeSystem value in a set of translations.  Since HL7 (or a government body) may mandate that codes from certain code systems be sent in conformant messages, other synonyms that are sent in the translation set need to be distinguished among the originally captured source, the HL7 specified code, or some future role.  When this code is NULL, it indicates that the translation is an undefined type.  When valued, this property must contain one of the following values: SRC - Source (or original) code HL7 - HL7 Specified or Mandated SH - both HL7 mandated and the original code (precoordination) There may be additional values added to this code system as we work through the use of codes in messages and determine other Use Cases requiring special interpretation of the translations.";
  dcterms:description " Identifies how to interpret the instance of the code, codeSystem value in a set of translations.  Since HL7 (or a government body) may mandate that codes from certain code systems be sent in conformant messages, other synonyms that are sent in the translation set need to be distinguished among the originally captured source, the HL7 specified code, or some future role.  When this code is NULL, it indicates that the translation is an undefined type.  When valued, this property must contain one of the following values: SRC - Source (or original) code HL7 - HL7 Specified or Mandated SH - both HL7 mandated and the original code (precoordination) There may be additional values added to this code system as we work through the use of codes in messages and determine other Use Cases requiring special interpretation of the translations.";
  dc:date "Mon Mar 23 00:00:00 EST 2015".

cs:CodingRationale.class a fhir:Concept;
  owl:oneOf (cs:CodingRationale\#O cs:CodingRationale\#OR cs:CodingRationale\#P cs:CodingRationale\#PR cs:CodingRationale\#R).

cs:CodingRationale.class\#O rdfs:subClassOf cs:CodingRationale.class;
  owl:oneOf (cs:CodingRationale\#O);
  rdfs:label "originally produced code";
  dc:title "originally produced code";
  rdfs:comment "Description: Originally produced code.";
  dcterms:description "Description: Originally produced code.".

cs:CodingRationale\#O a cs:CodingRationale.class\#O.

cs:CodingRationale.class\#OR rdfs:subClassOf cs:CodingRationale.class;
  owl:oneOf (cs:CodingRationale\#OR);
  rdfs:label "original and required";
  dc:title "original and required";
  rdfs:comment "Originally produced code, required by the specification describing the use of the coded concept.";
  dcterms:description "Originally produced code, required by the specification describing the use of the coded concept.".

cs:CodingRationale\#OR a cs:CodingRationale.class\#OR.

cs:CodingRationale.class\#P rdfs:subClassOf cs:CodingRationale.class;
  owl:oneOf (cs:CodingRationale\#P);
  rdfs:label "post-coded";
  dc:title "post-coded";
  rdfs:comment "Description: Post-coded from free text source</description>";
  dcterms:description "Description: Post-coded from free text source</description>".

cs:CodingRationale\#P a cs:CodingRationale.class\#P.

cs:CodingRationale.class\#PR rdfs:subClassOf cs:CodingRationale.class;
  owl:oneOf (cs:CodingRationale\#PR);
  rdfs:label "post-coded and required";
  dc:title "post-coded and required";
  rdfs:comment "Post-coded from free text source, required by the specification describing the use of the coded concept.";
  dcterms:description "Post-coded from free text source, required by the specification describing the use of the coded concept.".

cs:CodingRationale\#PR a cs:CodingRationale.class\#PR.

cs:CodingRationale.class\#R rdfs:subClassOf cs:CodingRationale.class;
  owl:oneOf (cs:CodingRationale\#R);
  rdfs:label "required";
  dc:title "required";
  rdfs:comment "Description: Required standard code for HL7.";
  dcterms:description "Description: Required standard code for HL7.".

cs:CodingRationale\#R a cs:CodingRationale.class\#R.

